ReprDepth as a ghost field
To enable complete abstraction when using an ADT to implement another
ADT, a ghost constant field is needed to hold ReprDepth, instead of
the old function.

src/linear/layer1/ADT.dfy
@@ -1,17 +1,15 @@
 trait ADT<M> {
-  function ReprDepth(): nat
-    ensures ReprDepth() > 0
+  ghost const ReprDepth: nat
 
   function ReprFamily(n: nat): set<object>
     decreases n
-    requires n <= ReprDepth()
     ensures n > 0 ==> ReprFamily(n) >= ReprFamily(n-1)
     reads this, if n == 0 then {} else ReprFamily(n-1)
 
   function Repr(): set<object>
-    reads this, ReprFamily(ReprDepth()-1)
+    reads this, if ReprDepth == 0 then {} else ReprFamily(ReprDepth-1)
   {
-    ReprFamily(ReprDepth())
+    ReprFamily(ReprDepth)
   }
 
   predicate Valid()
